imp/SimSTS2.v
@@ -13,6 +13,71 @@ Set Implicit Arguments.
 
 
 
+Section Beh.
+
+  Inductive match_val : eventval -> val -> Prop :=
+  | match_val_intro :
+      forall v, match_val (EVlong v) (Vint (Int64.signed v)).
+
+  Inductive match_event : Events.event -> Universe.event -> Prop :=
+  | match_event_intro
+      name eargs uargs er ur
+      (MV: Forall2 match_val eargs uargs)
+      (MV: match_val er ur)
+    :
+      match_event (Event_syscall name eargs er) (event_sys name uargs ur)
+  .
+
+  Variant _match_beh (match_beh: _ -> _ -> Prop) (tgtb : program_behavior) (srcb : Tr.t) : Prop :=
+  | match_beh_Terminates
+      tr mtr r
+      (MT : Forall2 match_event tr mtr)
+      (TB : tgtb = Terminates tr r)
+      (SB : srcb = Tr.app mtr (Tr.done r.(Int.intval)))
+    :
+      _match_beh match_beh tgtb srcb
+  | match_beh_Diverges
+      tr mtr
+      (MT : Forall2 match_event tr mtr)
+      (TB : tgtb = Diverges tr)
+      (SB : srcb = Tr.app mtr (Tr.spin))
+    :
+      _match_beh match_beh tgtb srcb
+  | match_beh_Reacts
+      ev mev trinf mtrinf
+      (ME : match_event ev mev)
+      (MB : match_beh (Reacts trinf) mtrinf)
+      (TB : tgtb = Reacts (Econsinf ev trinf))
+      (SB : srcb = Tr.cons mev mtrinf)
+    :
+      _match_beh match_beh tgtb srcb
+  | match_beh_ub_trace
+      mtr tr
+      (SB : srcb = Tr.app mtr (Tr.ub))
+      (MT : Forall2 match_event tr mtr)
+      (TB : behavior_prefix tr tgtb)
+    :
+      _match_beh match_beh tgtb srcb.
+
+  Definition match_beh : _ -> _ -> Prop := paco2 _match_beh bot2.
+
+  Lemma match_beh_mon : monotone2 _match_beh.
+  Proof.
+    ii. inv IN.
+    - econs 1; eauto.
+    - econs 2; eauto.
+    - econs 3; eauto.
+    - econs 4; eauto.
+  Qed.
+
+End Beh.
+Hint Constructors _match_beh.
+Hint Unfold match_beh.
+Hint Resolve match_beh_mon: paco.
+
+
+
+
 
 (************************ Coq Aux ****************************)
 (************************ Coq Aux ****************************)
@@ -839,7 +904,7 @@ Section SIM.
     ii. des; clarify. eapply SAFE; ss.
     { econs; et. }
     { instantiate (1 := e0 :: _). ss. des_ifs. rewrite MB0 in *; clarify. }
-    { esplits; et. }
+    { ss. }
   Qed.
 
   Lemma safe_along_events_step_none
@@ -933,7 +998,7 @@ Section SIM.
       exploit SAFE; try apply SRT.
       { econs; et. }
       { instantiate (1:=[]). ss. }
-      { esplits; et. }
+      { ss. }
       i; des.
       exploit wf_angelic; et. i; subst.
       exploit SIM0; et. i; des. pclearbot.
