imp/Imp.v
@@ -146,6 +146,7 @@ Section Denote.
 
     | Eq a b =>
       l <- denote_expr a ;; r <- denote_expr b ;;
+      (if (wf_val l && wf_val r) then Ret tt else triggerUB);;;
       match l, r with
       | Vint lv, Vint rv => if (lv =? rv)%Z then Ret (Vint 1) else Ret (Vint 0)
       | _, _ => triggerUB
